Move code

experiment/Experiment.Steel.Effect.fst
@@ -222,6 +222,11 @@ polymonadic_bind (PURE, MRepr) |> MRepr = bind_pure_mrepr
 
 (***** lifting Steel.Effect.SteelBase ~> MRepr *)
 
+/// The sub_effect is not working (order of resolution of the implicits, use of Steel's combinators instead of
+/// MRepr's combinators, Steel computation unexpectedly lifted where MRepr does not appear).
+/// One has use an explicit cast ([call]) instead.
+
+(*
 let lift_steel_mrepr
       (a : Type) (pre : SE.pre_t) (post : SE.post_t a)
       (req : SE.req_t pre) (ens : SE.ens_t pre a post)
@@ -231,6 +236,7 @@ let lift_steel_mrepr
       (fun () -> SE.SteelBase?.reflect f)
   
 sub_effect Steel.Effect.SteelBase ~> MRepr = lift_steel_mrepr
+*)
 
 unfold
 let call (#b : Type u#b)
@@ -240,7 +246,11 @@ let call (#b : Type u#b)
   : MRepr (a x) (M.Tspec (a x) (M.spec_r_steel u#a u#8 (pre x) (post x) (req x) (ens x)))
   = MRepr?.reflect (C.repr_of_steel #(a x) (pre x) (post x) (req x) (ens x) (fun () -> f x))
 
+
 (**** Conversion to Steel *)
+
+/// [ConvEffect] is a dummy effect whose only purpose is to avoid the retypechecking of [prog_tree] that would
+/// happen if it appeared outside effect combinators.
 
 type cv_repr (a : Type u#a) (pre : SE.pre_t) (post : SE.post_t a)
              (req : SE.req_t pre) (ens : SE.ens_t pre a post)
@@ -437,87 +447,17 @@ let mrepr_implicits_tac () : Tac unit
   )
 
 
-(**** Test *)
+(**** Notations *)
 
-open Steel.Effect.Common
-open Steel.Reference
-
-let display_term (#a : Type) (x : a) : Type = unit
-
-/// This retypecheck [r]. It fails if r contains a bind_pure since it will need to prove the monotonicity of the
-/// weakest precondition ([pure_wp_monotonic]).
-let dump_repr (#a : Type) (#r : prog_tree a)
-      ($re : unit -> MRepr a r)
-      (#[(norm [delta_attr [`%__repr_M__]; iota]; dump "dump_repr"; exact (`()))] d : display_term r)
-      ()
-  : unit
-  = ()
-
+unfold
+let usteel (a : Type) (pre : SE.pre_t) (post : SE.post_t a)
+          (req : SE.req_t pre) (ens : SE.ens_t pre a post)
+  : Type
+  = SH.unit_steel a pre post req ens
 
 let to_steel
       (#[apply (`[])] flags : list flag)
       (#a : Type) (#pre : SE.pre_t) (#post : SE.post_t a) (#req : SE.req_t pre) (#ens : SE.ens_t pre a post)
       (r : unit -> ConvEffect a pre post req ens flags)
-  : SH.unit_steel a pre post req ens
+  : usteel a pre post req ens
   = reify (r ())
-
-
-let test0 =
-  dump_repr (fun () -> let x = return 5 in return (x + 1)) ()
-
-//[@@ handle_smt_goals ] let tac () = Tactics.dump "SMT query"
-[@@ expect_failure [19]]
-let test1 = dump_repr (fun () -> assert (5 >= 0); return 5) ()
-
-let test1' (x : int)
-  : SH.unit_steel int emp (fun _ -> emp) (requires fun _ -> x >= 1) (ensures fun _ y _ -> y >= 5)
-  = to_steel #[Dump Stage_WP] begin fun () ->
-    assert (x >= 0);
-    return (5 + x)
-  end
-  
-
-let test2 (r : ref int) =
-  dump_repr (fun () -> let x = read r in return x) ()
-
-// Stack overflow
-//let test3 (b : bool) (r0 r1 : ref int) =
-//  dump_repr (fun () -> if b then let x = read r0 in return x
-//                         else let x = read r1 in return x)
-
-let test3' (b : bool) (r0 r1 : ref int)
-  : SH.unit_steel int (vptr r0 `star` vptr r1) (fun _ -> vptr r0 `star` vptr r1)
-         (requires fun h0 -> sel r0 h0 >= 0 /\ sel r1 h0 >= 0)
-         (ensures  fun h0 x h1 -> frame_equalities (vptr r0 `star` vptr r1) h0 h1 /\ x >= 0)
-  = to_steel #[Timer] begin fun () ->
-    if b then call read r0 else call read r1
-  end
-
-let test4 (r0 r1 : ref int) =
-  dump_repr (fun () ->
-    let x = read r0 in
-    write r1 (x + 1);
-    return ())
-  ()
-
-// Fails because the prog_tree contains some uvar (because the Steel's tactic is called after our tactic ?)
-[@@ expect_failure [228]]
-let test5 (r : ref nat)
-  : SH.unit_steel unit
-      (vptr r) (fun _ -> vptr r)
-      (requires fun h0 -> sel r h0 > 10) (ensures fun _ _ h1 -> sel r h1 >= 10)
-  = to_steel #[Dump Stage_M] begin fun () ->
-    let x = read r in
-    let _ = return () in
-    write r (x - 1);
-    return ()
-  end
-
-let test5' (r : ref nat)
-  : SH.unit_steel unit
-      (vptr r) (fun _ -> vptr r)
-      (requires fun h0 -> sel r h0 > 10) (ensures fun _ _ h1 -> sel r h1 >= 10)
-  = to_steel begin fun () ->
-    let x = call read r in
-    call (write r) (x - 1)
-  end
