experiment/Experiment.Steel.fst
@@ -1,16 +1,61 @@
 module Experiment.Steel
 
-module SF     = Experiment.Steel.Repr.SF
+/// Entry point for the functionalisation of Steel programs
+
+module U    = Learn.Util
+module L    = FStar.List.Pure
+module SE   = Steel.Effect
+module SH   = Experiment.Steel.Steel
+module Ll   = Learn.List
+module Dl   = Learn.DList
+module Fl   = Learn.FList
+module UV   = Learn.Universe
+module Msk  = Learn.List.Mask
+module Perm = Learn.Permutation
+
+module M   = Experiment.Steel.Repr.M
+module ST  = Experiment.Steel.Repr.ST
+module LV  = Experiment.Steel.Repr.LV
+module SF  = Experiment.Steel.Repr.SF
+module Fun = Experiment.Repr.Fun
+module Vpl = Experiment.Steel.VPropList
+module Veq = Experiment.Steel.VEquiv
+
+module TcS  = Experiment.Steel.Tac
+module TcM  = Experiment.Steel.Tac.MCond
+module TcLV = Experiment.Steel.Tac.LV
+
+module LV2M   = Experiment.Steel.Repr.LV_to_M
+module LV2SF  = Experiment.Steel.Repr.LV_to_SF
 module SF2Fun = Experiment.Steel.Repr.SF_to_Fun
 
+open FStar.Tactics
+open Learn.Tactics.Util
+open Experiment.Steel.Interface
 
-#set-options "--ide_id_info_off --ifuel 0"
 
-(**) #push-options "--ifuel 0"
-(**) private let __begin_prog_to_Fun = ()
-(**) #pop-options
-(**) private let __end_prog_to_Fun = ()
+/// Here, [lc] should be the [lin_cond] obtained from [LV.lc_sub_push]
+let prog_LV_to_Fun
+      (#a : Type) (t : M.prog_tree a)
+      (#pre : M.pre_t) (#post : M.post_t a)
+      (lc : LV.top_lin_cond t pre post)
+      (sl0 : Vpl.sl_f pre)
+  : Fun.prog_tree #SF2Fun.sl_tys SF.({val_t = a; sel_t = M.post_sl_t post})
+  =
+    let t_SF = LV2SF.repr_SF_of_LV lc (Fl.dlist_of_f sl0) in
+    SF2Fun.repr_Fun_of_SF t_SF
 
+let prog_M_equiv_Fun 
+      (#a : Type) (t : M.prog_tree a)
+      (#pre : M.pre_t) (#post : M.post_t a)
+      (c : M.tree_cond t pre post)
+      (sl0 : Vpl.sl_f pre)
+      (f : Fun.prog_tree #SF2Fun.sl_tys SF.({val_t = a; sel_t = M.post_sl_t post}))
+  : prop
+  = (M.tree_req t c sl0 <==> Fun.tree_req f) /\
+    (M.tree_req t c sl0 ==>
+    (forall (x : a) (sl1 : Vpl.sl_f (post x)) .
+        M.tree_ens t c sl0 x sl1 <==> Fun.tree_ens f ({val_v = x; sel_v = sl1})))
 
 #push-options "--ifuel 0 --fuel 0"
 let prog_LV_to_Fun_equiv_M
@@ -41,7 +86,369 @@ let prog_LV_to_Fun_equiv_M
             let _ = mintros () in apply_lemma (``@lem_ens))
 #pop-options
 
-(**) #push-options "--no_tactics"
-(**) private let __begin_build_to_steel_wrew = ()
-(**) #pop-options
-(**) private let __end_build_to_steel_wrew = ()
+inline_for_extraction
+let prog_LV_to_Fun_extract
+      (#a : Type) (t : M.repr SH.KSteel a)
+      (#pre : M.pre_t) (#post : M.post_t a)
+      (lc : LV.top_lin_cond t.repr_tree pre post {LV.lcsub_at_leaves lc})
+      (req : M.req_t pre) (ens : M.ens_t pre a post)
+      (sub : (sl0 : Vpl.sl_f pre) -> Lemma (requires req sl0)
+               (ensures Fun.tree_req (prog_LV_to_Fun t.repr_tree lc sl0) /\
+                  (forall (x : a) (sl1 : Vpl.sl_f (post x)) .
+                    Fun.tree_ens (prog_LV_to_Fun t.repr_tree lc sl0) SF.({val_v = x; sel_v = sl1}) ==>
+                    ens sl0 x sl1)))
+  : M.repr_steel_t SH.KSteel a pre post req ens
+  =
+    let tr = t.repr_tree in
+    let mc = LV2M.repr_M_of_LV_top lc in
+    U.cast _ (M.repr_steel_subcomp _ _ req ens
+      (fun sl0       -> let _ =
+        let f = prog_LV_to_Fun t.repr_tree lc sl0 in
+        sub sl0;
+        prog_LV_to_Fun_equiv_M t.repr_tree lc sl0;
+        // Probably because of [U.eta], the SMT fails to solve this. We rely on tactics instead.
+        assert (prog_M_equiv_Fun tr mc sl0 f ==> (M.tree_req tr mc sl0 <==> Fun.tree_req f))
+          by (hyp (destruct_and (implies_intro ()))._1)
+        in ())
+      (fun sl0 x sl1 -> let _ =
+        let f = prog_LV_to_Fun t.repr_tree lc sl0 in
+        prog_LV_to_Fun_equiv_M t.repr_tree lc sl0;
+        assert (prog_M_equiv_Fun tr mc sl0 f ==> M.tree_req tr mc sl0 ==>
+          (M.tree_ens tr mc sl0 x sl1 <==> Fun.tree_ens f ({val_v = x; sel_v = sl1})))
+          by (let eqv = (destruct_and (implies_intro ()))._2 in
+              let req = implies_intro () in
+              let eqv = instantiate (binder_to_term eqv) (binder_to_term req) in
+              let eqv = instantiate (binder_to_term eqv) (``@x) in
+              let eqv = instantiate (binder_to_term eqv) (``@sl1) in
+              hyp eqv);
+        sub sl0
+        in ())
+      (t.repr_steel pre (U.eta post) mc))
+
+inline_for_extraction
+let prog_LV_to_Fun_extract_wp
+      (#a : Type) (t : M.repr SH.KSteel a)
+      (#pre : M.pre_t) (#post : M.post_t a)
+      (lc0 : LV.top_lin_cond t.repr_tree pre post)
+      (lc1 : LV.top_lin_cond t.repr_tree pre post) (_ : squash (lc1 == LV.lc_sub_push lc0))
+      (req : M.req_t pre) (ens : M.ens_t pre a post)
+      (wp : (sl0 : Vpl.sl_f pre) -> Lemma
+              (requires req sl0)
+              (ensures Fun.tree_wp (prog_LV_to_Fun t.repr_tree lc1 sl0) (fun res -> ens sl0 res.val_v res.sel_v)))
+  : M.repr_steel_t SH.KSteel a pre post req ens
+  =
+    (**) LV.lc_sub_push_at_leaves _ lc0;
+    prog_LV_to_Fun_extract t lc1 req ens
+      (fun sl0 -> wp sl0;
+               Fun.tree_wp_sound (prog_LV_to_Fun t.repr_tree lc1 sl0) (fun res -> ens sl0 res.val_v res.sel_v))
+
+
+(**** normalisation steps *)
+
+let __normal_M : list norm_step = [
+  delta_only [`%Vpl.vprop_list_sels_t;   `%M.Mkrepr?.repr_tree;
+              `%L.map; `%SE.Mkvprop'?.t; `%UV.lift_dom];
+  delta_attr [`%__tac_helper__; `%__repr_M__; `%SE.__reduce__];
+  delta_qualifier ["unfold"];
+  iota; zeta
+]
+
+let __normal_lc_sub_push : list norm_step = [
+  delta_only (L.append TcS.__delta_list
+             [`%LV.lc_sub_push; `%LV.lc_sub_push_aux; `%LV.lcsubp_tr;
+              `%Perm.perm_f_to_list; `%Perm.perm_f_of_list;
+              `%Perm.comp; `%Perm.mk_perm_f; `%Perm.perm_f_append; `%Perm.perm_f_cons; `%Perm.id_n;
+              `%Perm.perm_f_cons_snoc]);
+  delta_attr [`%LV.__lin_cond__; `%Msk.__mask__; `%__tac_helper__];
+  delta_qualifier ["unfold"];
+  iota; zeta; primops
+]
+
+let __normal_LV2SF : list norm_step = [
+  delta_only [`%prog_LV_to_Fun; `%LV2SF.repr_SF_of_LV;
+              `%Vpl.filter_sl;
+              `%M.post_sl_t; `%Vpl.vprop_list_sels_t;
+              `%L.map; `%L.op_At; `%L.append; `%Ll.initi; `%L.length; `%Ll.repeat;
+              `%Dl.initi; `%Dl.append; `%Dl.index; `%Dl.dlist_eq2; `%Msk.dl_append_on_mask;
+              `%Fl.dlist_of_f; `%Fl.flist_eq2;
+              `%Fl.append; `%Fl.splitAt_ty;
+              `%Mktuple2?._1; `%Mktuple2?._2];
+  delta_attr [`%__LV2SF__; `%LV.__lin_cond__; `%Msk.__mask__; `%__tac_helper__; `%SE.__reduce__];
+  delta_qualifier ["unfold"];
+  iota; zeta; primops
+]
+
+let __normal_Fun : list norm_step = [
+  delta_only [`%SF2Fun.repr_Fun_of_SF;
+              `%SF2Fun.shape_Fun_of_SF; `%SF.Mkprog_shape?.post_len; `%SF.Mkprog_shape?.shp];
+  delta_qualifier ["unfold"];
+  iota; zeta; primops
+]
+
+let __normal_Fun_elim_returns_0 : list norm_step = [
+  delta_only [`%Fun.elim_returns; `%Fun.elim_returns_aux; `%Fun.elim_returns_k_trm; `%Fun.elim_returns_k_ret;
+              `%SF2Fun.sl_tys; `%SF2Fun.sl_tys_lam;
+              `%Fun.Mktys'?.v_of_r; `%Fun.Mktys'?.r_of_v;
+              `%Fun.Mktys_lam'?.lam_prop; `%Fun.Mktys_lam'?.lam_tree;
+              `%SF2Fun.Mksl_tys_t?.val_t; `%SF2Fun.Mksl_tys_t?.sel_t;
+              `%SF2Fun.Mksl_tys_v?.val_v; `%SF2Fun.Mksl_tys_v?.sel_v;
+              `%SF2Fun.Mksl_tys_r?.vl;    `%SF2Fun.Mksl_tys_r?.sl;
+              `%Fun.Tret?.x;
+              `%SF2Fun.sl_r_of_v; `%SF2Fun.sl_v_of_r;
+              `%Fl.cons; `%Fl.nil; `%Fl.dlist_of_f; `%Fl.flist_of_d'; `%Dl.initi; `%Dl.index;
+              `%L.length; `%L.index; `%L.hd; `%L.tl; `%L.tail; `%Ll.initi
+              ];
+  delta_qualifier ["unfold"];
+  iota; zeta; primops
+]
+
+let __normal_Fun_elim_returns_1 : list norm_step = [
+  delta_only [`%SF2Fun.delayed_sl_uncurrify];
+  delta_qualifier ["unfold"];
+  iota; zeta; primops
+]
+
+let __normal_Fun_spec : list norm_step = [
+  delta_only [`%Fun.tree_wp; `%Fl.partial_app_flist;
+              `%Fun.Mktys'?.all; `%SF2Fun.sl_tys; `%SF2Fun.sl_all; `%Fl.forall_flist;
+              `%Fun.Mktys'?.v_of_r; `%SF2Fun.sl_v_of_r; `%Fl.flist_of_d';
+              `%Fl.cons; `%Fl.nil;
+              `%SF2Fun.Mksl_tys_t?.val_t; `%SF2Fun.Mksl_tys_t?.sel_t;
+              `%SF2Fun.Mksl_tys_v?.val_v; `%SF2Fun.Mksl_tys_v?.sel_v;
+              `%SF2Fun.Mksl_tys_r?.vl;    `%SF2Fun.Mksl_tys_r?.sl;
+              `%Vpl.vprop_of_list; `%Vpl.vprop_of_list'];
+  delta_qualifier ["unfold"];
+  delta_attr [`%SE.__steel_reduce__; `%Msk.__mask__; `%UV.__universe__];
+  iota; zeta; primops
+]
+
+let __normal_vprop_list : list norm_step = [
+  delta_only [`%Vpl.vprop_of_list; `%Vpl.vprop_list_sels_t;
+              `%Fl.flist_of_g; `%Fl.dlist_of_f_g; `%Fl.flist_of_d;
+              `%Dl.index; `%Dl.initi_g;
+              `%L.length; `%L.index; `%L.map; `%L.hd; `%L.tl; `%L.tail];
+  delta_attr [`%SE.__reduce__];
+  iota; zeta; primops
+]
+
+let __normal_extract : list norm_step = [
+  delta_qualifier ["inline_for_extraction"; "unfold"];
+  iota; zeta; primops
+]
+
+
+(***** Extracting a [M.repr_steel_t] from a [M.repr] *)
+
+/// We mention [t] so that it is specified by the goal, but this type is just a synonym for [M.repr_steel_t].
+let extract (a : Type) (pre : M.pre_t) (post : M.post_t a) (req : M.req_t pre) (ens : M.ens_t pre a post)
+            (t : M.repr SH.KSteel a)
+  : Type
+  = M.repr_steel_t SH.KSteel a pre post req ens
+
+[@@ __tac_helper__]
+inline_for_extraction
+let __solve_by_wp_LV
+      (#a : Type) (t : M.repr SH.KSteel a)
+      (#pre : M.pre_t) (#post : M.post_t a)
+      (#req : M.req_t pre) (#ens : M.ens_t pre a post)
+      (lc0 : LV.top_lin_cond t.repr_tree pre post)
+      (lc1 : LV.top_lin_cond t.repr_tree pre post) (lc1_eq : squash (lc1 == LV.lc_sub_push lc0))
+      (t_Fun : (sl0 : Vpl.sl_f pre) ->
+               GTot (Fun.prog_tree #SF2Fun.sl_tys ({val_t = a; sel_t = M.post_sl_t post})))
+      (t_Fun_eq : squash (t_Fun == (fun sl0 -> prog_LV_to_Fun t.repr_tree lc1 sl0)))
+      (wp : squash (Fl.forall_flist (Vpl.vprop_list_sels_t pre) (fun sl0 ->
+               req sl0 ==>
+               Fun.tree_wp (t_Fun sl0) (fun res -> ens sl0 res.val_v res.sel_v))))
+      (ext : M.repr_steel_t SH.KSteel a pre post req ens)
+      (ext_eq : ext == prog_LV_to_Fun_extract_wp t lc0 lc1 lc1_eq req ens (fun sl0 -> ()))
+  : extract a pre post req ens t
+  =
+    ext
+
+/// Solves a goal of the form [extract a pre post req ens t]
+let solve_by_wp (fr : flags_record) (t : timer) : Tac unit
+  =
+    apply_raw (`__solve_by_wp_LV);
+    
+    (* lc0 *)
+    let t = timer_enter t "lin_cond  " in
+    norm __normal_M;
+    if fr.f_dump Stage_M then dump1 "at stage M";
+    TcLV.build_top_lin_cond fr;
+
+    (* lc1 *)
+    let t = timer_enter t "sub_push  " in
+    dismiss ();
+    TcLV.norm_lc ();
+    if fr.f_dump (Stage_LV false) then dump1 "at stage LV (before sub_push)";
+    norm __normal_lc_sub_push;
+    if fr.f_dump (Stage_LV  true) then dump1 "at stage LV (after sub_push)";
+    trefl ();
+
+    (* t_Fun *)
+    dismiss ();
+    let t = timer_enter t "LV2SF     " in
+    norm __normal_LV2SF;
+    if fr.f_dump Stage_SF then dump1 "at stage SF";
+    let t = timer_enter t "SF2Fun    " in
+    norm __normal_Fun;
+    if fr.f_dump Stage_Fun then dump1 "at stage Fun";
+    trefl ();
+
+    (* wp *)
+    let t = timer_enter t "Fun_wp    " in
+    norm __normal_M;
+    norm __normal_Fun_spec;
+    if fr.f_dump Stage_WP then dump1 "at stage WP";
+    smt ();
+
+    (* ext *)
+    dismiss ();
+    let t = if fr.f_extr then begin
+      // We normalize the resulting Steel program so that it can be extracted
+      let t = timer_enter t "extract   " in
+      norm __normal_extract;
+      t
+    end else t in
+    if fr.f_dump Stage_Extract then dump1 "at stage Extract";
+    trefl ();
+    timer_stop t
+
+
+(***** Extracting a [unit_steel] from a [M.repr] *)
+
+/// Similarly to [extract], [t] is only mentioned so that it can be retrieved by the tactic
+type __to_steel_goal
+      (a : Type) (pre : SE.pre_t) (post : SE.post_t a) (req : SE.req_t pre) (ens : SE.ens_t pre a post)
+      (t : M.repr SH.KSteel a)
+  = SH.unit_steel a pre post req ens
+
+[@@ __tac_helper__]
+inline_for_extraction
+let __build_to_steel
+      (#a : Type) (#pre : SE.pre_t) (#post : SE.post_t a) (#req : SE.req_t pre) (#ens : SE.ens_t pre a post)
+      (#t : M.repr SH.KSteel a)
+      (goal_tr : M.to_repr_t a pre post req ens)
+      (goal_f  : extract a goal_tr.r_pre goal_tr.r_post goal_tr.r_req goal_tr.r_ens t)
+  : __to_steel_goal a pre post req ens t
+  = M.steel_of_repr goal_tr goal_f
+
+/// Solves a goal [__to_steel_goal]
+let build_to_steel (fr : flags_record) : Tac unit
+  =
+    // This tactics fails if called in lax mode.
+    // It appears that at this point the goal contains unification variables in lax-mode:
+    //   __to_steel_goal unit ?pre ?post ?req ?ens t
+    // whereas the specifications are concrete terms (inferred from the top-level annotation) in normal-mode.
+    // If we try to solve the goal with [lax_guard], we obtain:
+    //   (Error 217) Tactic left uninstantiated unification variable ?421 of type Type
+    //               (reason = "Instantiating implicit argument in application")
+    with_policy Force (fun () ->
+    let t = timer_start "specs     " fr.f_timer in
+    apply_raw (`__build_to_steel);
+    TcS.build_to_repr_t fr (fun () -> [Info_location "in the specification"]);
+
+    // [extract]
+    norm [delta_attr [`%__tac_helper__]; iota];
+    solve_by_wp fr t
+    )
+
+
+[@@ __tac_helper__]
+inline_for_extraction
+let to_steel
+      (#a : Type) (#pre : SE.pre_t) (#post : SE.post_t a) (#req : SE.req_t pre) (#ens : SE.ens_t pre a post)
+      (t : M.repr SH.KSteel a)
+      (g : __to_steel_goal a pre post req ens t)
+  : SH.unit_steel a pre post req ens
+  = g
+
+
+(***** Using a [rewrite_with_tactic] *)
+
+noeq
+type to_steel_goal_spec
+      (a : Type) (pre : M.pre_t) (post : M.post_t a) (req : M.req_t pre) (ens : M.ens_t pre a post)
+      (t : M.prog_tree a)
+  = {
+    goal_spec_LV : LV.top_lin_cond t pre post;
+    goal_spec_WP : squash (
+      let lc1 = LV.lc_sub_push goal_spec_LV in
+      let t_Fun sl0 = prog_LV_to_Fun t lc1 sl0 in
+     (forall (sl0 : Vpl.sl_f pre) .
+       req sl0 ==>
+       Fun.tree_wp (t_Fun sl0) (fun res -> ens sl0 res.val_v res.sel_v))
+    )
+  }
+
+let to_steel_goal_spec_WP
+      (a : Type) (pre : M.pre_t) (post : M.post_t a) (req : M.req_t pre) (ens : M.ens_t pre a post)
+      (t : M.prog_tree a)
+      (lc0 : LV.top_lin_cond t pre post)
+  : Type0
+  =
+    let lc1 = LV.lc_sub_push lc0 in
+    let t_Fun sl0 = prog_LV_to_Fun t lc1 sl0 in
+    Fl.forall_flist (Vpl.vprop_list_sels_t pre) (fun (sl0 : Vpl.sl_f pre) ->
+       req sl0 ==>
+       Fun.tree_wp (t_Fun sl0) (fun res -> ens sl0 res.val_v res.sel_v))
+
+private
+let rewrite_to_steel_goal_spec (flags : list flag) () : Tac unit
+  =
+    let fr = make_flags_record flags in
+    norm [delta_only [`%to_steel_goal_spec_WP]];
+    
+    let t = timer_start "sub_push  " fr.f_timer in
+    TcLV.norm_lc ();
+    if fr.f_dump (Stage_LV false) then dump1 "at stage LV (before sub_push)";
+    norm __normal_lc_sub_push;
+    if fr.f_dump (Stage_LV  true) then dump1 "at stage LV (after sub_push)";
+    
+    let t = timer_enter t "LV2SF     " in
+    norm __normal_LV2SF;
+    if fr.f_dump Stage_SF then dump1 "at stage SF";
+    
+    let t = timer_enter t "SF2Fun    " in
+    norm __normal_Fun;
+    if fr.f_dump Stage_Fun then dump1 "at stage Fun";
+    
+    let t = timer_enter t "Fun_wp    " in
+    norm __normal_M;
+    norm __normal_Fun_spec;
+    if fr.f_dump Stage_WP then dump1 "at stage WP";
+
+    trefl ();
+    timer_stop t
+
+#push-options "--no_tactics"
+private
+let __build_to_steel_wrew
+      (flags : list flag)
+      (a : Type) (pre : M.pre_t) (post : M.post_t a) (req : M.req_t pre) (ens : M.ens_t pre a post)
+      (t : M.prog_tree a)
+      (goal_LV : LV.top_lin_cond t pre post)
+      (goal_WP : squash (rewrite_with_tactic (rewrite_to_steel_goal_spec flags)
+                         (to_steel_goal_spec_WP a pre post req ens t goal_LV)))
+  : to_steel_goal_spec a pre post req ens t
+  =
+    unfold_rewrite_with_tactic
+        (rewrite_to_steel_goal_spec flags)
+        (to_steel_goal_spec_WP a pre post req ens t goal_LV);
+    Mkto_steel_goal_spec goal_LV goal_WP
+#pop-options
+
+let build_to_steel_wrew (fr : flags_record) (flags : list flag) (t : timer) : Tac timer
+  =
+    apply_raw (`__build_to_steel_wrew (`#(quote flags)));
+    
+    // goal_LV
+    let t = timer_enter t "lin_cond  " in
+    norm __normal_M;
+    if fr.f_dump Stage_M then dump1 "at stage M";
+    TcLV.build_top_lin_cond fr;
+
+    // goal_WP
+    smt ();
+
+    t
