experiment/Experiment.Steel.Effect.Test.fst
@@ -1,0 +1,80 @@
+module Experiment.Steel.Effect.Test
+
+open FStar.Tactics
+open Steel.Effect.Common
+open Steel.Reference
+open Experiment.Steel.Interface
+open Experiment.Steel.Effect
+
+let display_term (#a : Type) (x : a) : Type = unit
+
+/// This retypecheck [r]. It fails if r contains a bind_pure since it will need to prove the monotonicity of the
+/// weakest precondition ([pure_wp_monotonic]).
+let dump_repr (#a : Type) (#r : prog_tree a)
+      ($re : unit -> MRepr a r)
+      (#[(norm [delta_attr [`%__repr_M__]; iota]; dump "dump_repr"; exact (`()))] d : display_term r)
+      ()
+  : unit
+  = ()
+
+
+let test0 =
+  dump_repr (fun () -> let x = return 5 in return (x + 1)) ()
+
+//[@@ handle_smt_goals ] let tac () = Tactics.dump "SMT query"
+[@@ expect_failure [19]]
+let test1 = dump_repr (fun () -> assert (5 >= 0); return 5) ()
+
+let test1' (x : int)
+  : usteel int emp (fun _ -> emp) (requires fun _ -> x >= 1) (ensures fun _ y _ -> y >= 5)
+  = to_steel #[Dump Stage_WP] begin fun () ->
+    assert (x >= 0);
+    return (5 + x)
+  end
+  
+
+//let test2 (r : ref int) =
+//  dump_repr (fun () -> let x = call read r in return x) ()
+
+// Stack overflow
+//let test3 (b : bool) (r0 r1 : ref int) =
+//  dump_repr (fun () -> if b then let x = read r0 in return x
+//                         else let x = read r1 in return x)
+
+let test3' (b : bool) (r0 r1 : ref int)
+  : usteel int (vptr r0 `star` vptr r1) (fun _ -> vptr r0 `star` vptr r1)
+         (requires fun h0 -> sel r0 h0 >= 0 /\ sel r1 h0 >= 0)
+         (ensures  fun h0 x h1 -> frame_equalities (vptr r0 `star` vptr r1) h0 h1 /\ x >= 0)
+  = to_steel #[Timer] begin fun () ->
+    if b then call read r0 else call read r1
+  end
+
+//let test4 (r0 r1 : ref int) =
+//  dump_repr (fun () ->
+//    let x = call read r0 in
+//    call (write r1) (x + 1);
+//    return ())
+//  ()
+
+// With the sub_effect Steel ~> MRepr, fails because the prog_tree contains some uvar
+// (because the Steel's tactic is called after our tactic ?)
+//[@@ expect_failure [228]]
+//let test5 (r : ref nat)
+//  : usteel unit
+//      (vptr r) (fun _ -> vptr r)
+//      (requires fun h0 -> sel r h0 > 10) (ensures fun _ _ h1 -> sel r h1 >= 10)
+//  = to_steel #[Dump Stage_M] begin fun () ->
+//    let x = read r in
+//    let _ = return () in
+//    write r (x - 1);
+//    return ()
+//  end
+
+let test5' (r : ref nat)
+  : usteel unit
+      (vptr r) (fun _ -> vptr r)
+      (requires fun h0 -> sel r h0 > 10) (ensures fun _ _ h1 -> sel r h1 >= 10)
+  = to_steel begin fun () ->
+    let x = call read r in
+    call (write r) (x - 1)
+  end
